theories/CertiGC/vst/proof/verif_do_scan.v
@@ -400,15 +400,16 @@ Proof.
                  destruct H38 as [? [? [? ?]]].
                  assert (heapgraph_generation_base g3 from = heapgraph_generation_base g4 from) by
                      (eapply fr_gen_start; eauto).
-                 assert (limit_address g3 t_info3 from =
-                         limit_address g4 t_info4 from). {
+                 assert (limit_address g3 t_info3 from = limit_address g4 t_info4 from).
+                {
                    unfold limit_address.
                    rewrite H45.
                    do 2 f_equal.
-                   now rewrite (proj1 (proj2 H42)), (thread_info_relation__space_remembered _ _ _ H42).
-                 }
+                   (* now rewrite (proj1 (proj2 H42)), (thread_info_relation__space_remembered _ _ _ H42). *)
+                   admit. (* TIM TODO: we need to prove that space_remembered is unchanged *)
+                }
                  assert (next_address t_info3 to = next_address t_info4 to) by
-                     (unfold next_address; f_equal; apply (proj1 H42)). entailer!.
+                     (unfold next_address; f_equal; apply (thread_info_relation__ti_heap H42)). entailer!.
                  split; [|split; [|split]]; try easy.
                  --- remember (nat_inc_list
                                  (Datatypes.length
